pulse/share/steel/examples/pulse/lib/Pulse.Lib.HashTable.fst
@@ -64,7 +64,7 @@ let pht_sz #k #v (pht:pht_t k v) : GTot pos = pht.repr.sz
 fn alloc (#k:eqtype) (#v:Type0) (hashf:(k -> SZ.t)) (l:pos_us)
   requires emp
   returns ht:ht_t k v
-  ensures exists* pht. models ht pht  ** pure (pht == mk_init_pht hashf l)
+  ensures exists* pht. models ht pht ** pure (pht == mk_init_pht hashf l)
 {
   let contents = V.alloc #(cell k v) Clean l;
   let ht = mk_ht l hashf contents;
@@ -103,8 +103,11 @@ let size_t_mod (x:SZ.t) (y : SZ.t { y =!= 0sz })
 : z:SZ.t { SZ.v z == SZ.v x % SZ.v y }
   = SZ.(x %^ y)
 
+noextract
+let same_sz_and_hashf (#kt:eqtype) (#vt:Type) (ht1 ht2:ht_t kt vt) : GTot prop =
+  ht1.sz == ht2.sz /\
+  ht1.hashf == ht2.hashf
 
-// #push-options "--admit_smt_queries true"
 ```pulse
 fn replace (#kt:eqtype) (#vt:Type)
   (#pht:erased (pht_t kt vt))
@@ -117,39 +120,37 @@ fn replace (#kt:eqtype) (#vt:Type)
   requires models ht pht
   returns p:(ht_t kt vt & vt)
   ensures models (fst p) (PHT.upd_pht #kt #vt pht idx k v ()) **
-          pure ((fst p).sz == ht.sz /\ (fst p).hashf == ht.hashf /\ Some (snd p) == PHT.lookup pht k)
+          pure (same_sz_and_hashf (fst p) ht /\ Some (snd p) == PHT.lookup pht k)
 {
   let hashf = ht.hashf;
   let mut contents = ht.contents;
   unfold models;
-  assert (R.pts_to contents ht.contents);
   rewrite (R.pts_to contents ht.contents) as (R.pts_to contents (reveal (hide ht.contents)));
   rewrite (V.pts_to ht.contents pht.repr.seq) as (V.pts_to (reveal (hide ht.contents)) pht.repr.seq);
-  // show_proof_state;
-  // with s. rewrite (V.pts_to ht.contents s) as (V.pts_to vcontents s);
-  // show_proof_state;
-  let v' = V.replace_ref contents idx (mk_used_cell k v);
+  let v' = V.replace_i_ref contents idx (mk_used_cell k v);
   let vcontents = !contents;
-  let ht1 = { sz = ht.sz; hashf = hashf; contents = vcontents };
+  let ht1 = mk_ht ht.sz hashf vcontents;
   with s. rewrite (V.pts_to (reveal (hide ht.contents)) s) as (V.pts_to ht1.contents s);
-  fold (models ht1 (PHT.upd_pht #kt #vt pht idx k v ()));
-  assert (pure (Used? v'));
+  fold (models ht1 (PHT.upd_pht pht idx k v ()));
   match v' {
     Used k' v' -> {
-      let res = (ht1, v');
+      let res = ((ht1 <: ht_t kt vt), v');
       with pht. rewrite (models ht1 pht) as (models (fst res) pht);
-      admit ();
       res
     }
-    _ -> { admit () }
+    Clean -> {
+      assert (pure (Used? v'));
+      Pulse.Lib.Core.unreachable ()
+    }
+    Zombie -> {
+      assert (pure (Used? v'));
+      Pulse.Lib.Core.unreachable ()
+    }
   }
 }
 ```
-// #pop-options
 
-#set-options "--print_implicits"
-
-#push-options "--z3rlimit_factor 8"
+#push-options "--fuel 1 --ifuel 1"
 ```pulse
 fn lookup (#kt:eqtype) (#vt:Type0) (#pht:erased (pht_t kt vt))
   (ht:ht_t kt vt)
@@ -157,7 +158,7 @@ fn lookup (#kt:eqtype) (#vt:Type0) (#pht:erased (pht_t kt vt))
   requires models ht pht
   returns  p:(ht_t kt vt & bool & option SZ.t)
   ensures  models (tfst p) pht ** 
-           pure ((tfst p).sz == ht.sz /\ (tfst p).hashf == ht.hashf /\ (tsnd p ==> tthd p == PHT.lookup_index_us pht k))
+           pure (same_sz_and_hashf (tfst p) ht /\ (tsnd p ==> tthd p == PHT.lookup_index_us pht k))
 {
   open SZ;
 
@@ -170,7 +171,7 @@ fn lookup (#kt:eqtype) (#vt:Type0) (#pht:erased (pht_t kt vt))
   let mut err = false;
   let mut ret = None #SZ.t;
   unfold (models ht pht);
-  // with s. rewrite (V.pts_to ht.contents s) as (V.pts_to contents s);
+
   while (let voff = !off;
          let vcont = !cont;
          let verr = !err; 
@@ -205,7 +206,7 @@ fn lookup (#kt:eqtype) (#vt:Type0) (#pht:erased (pht_t kt vt))
         Some sum -> 
         {
           let idx = size_t_mod sum ht.sz;
-          let c = V.replace_ref contents idx Zombie; 
+          let c = V.replace_i_ref contents idx Zombie; 
           match c
           {
             Used k' v' ->
@@ -214,7 +215,7 @@ fn lookup (#kt:eqtype) (#vt:Type0) (#pht:erased (pht_t kt vt))
               {
                 cont := false;
                 ret := Some idx;
-                V.replace_ref contents idx (Used k' v');
+                V.replace_i_ref contents idx (Used k' v');
                 with vcontents. assert (R.pts_to contents vcontents);
                 with s. assert (V.pts_to vcontents s);
                 assert (pure (Seq.equal s pht.repr.seq));
@@ -223,7 +224,7 @@ fn lookup (#kt:eqtype) (#vt:Type0) (#pht:erased (pht_t kt vt))
               } else
               {
                 off := voff +^ 1sz;
-                V.replace_ref contents idx (Used k' v');
+                V.replace_i_ref contents idx (Used k' v');
                 with vcontents. assert (R.pts_to contents vcontents);
                 with s. assert (V.pts_to vcontents s);
                 assert (pure (Seq.equal s pht.repr.seq));
@@ -234,7 +235,7 @@ fn lookup (#kt:eqtype) (#vt:Type0) (#pht:erased (pht_t kt vt))
             Clean ->
             {
               cont := false;
-              V.replace_ref contents idx c;
+              V.replace_i_ref contents idx c;
               with vcontents. assert (R.pts_to contents vcontents);
               with s. assert (V.pts_to vcontents s);
               assert (pure (Seq.equal s pht.repr.seq));
@@ -244,7 +245,7 @@ fn lookup (#kt:eqtype) (#vt:Type0) (#pht:erased (pht_t kt vt))
             Zombie ->
             {
               off := voff +^ 1sz;
-              V.replace_ref contents idx c;
+              V.replace_i_ref contents idx c;
               with vcontents. assert (R.pts_to contents vcontents);
               with s. assert (V.pts_to vcontents s);
               assert (pure (Seq.equal s pht.repr.seq));
@@ -269,107 +270,25 @@ fn lookup (#kt:eqtype) (#vt:Type0) (#pht:erased (pht_t kt vt))
   with vcontents_g. assert (R.pts_to contents vcontents_g);
   rewrite (V.pts_to vcontents_g pht.repr.seq) as (V.pts_to ht.contents pht.repr.seq);
   fold (models ht pht);
-  // with s. rewrite (V.pts_to contents s) as (V.pts_to ht.contents s);
-  // fold (models ht pht);
-
-  // let ht = mk_ht ht.sz ht.hashf contents;
   if verr
   {
-    let res = (ht, false, o);
-    admit ();
+    let res = ((ht <: ht_t kt vt), false, o);
     rewrite (models ht pht) as (models (tfst res) pht);
     res
   }
   else
   {
-    let res = (ht, true, o);
+    let res = ((ht <: ht_t kt vt), true, o);
     assert (R.pts_to ret (PHT.lookup_index_us pht k));
-    admit ();
     rewrite (models ht pht) as (models (tfst res) pht);
-    (ht, true, o)
+    res
   }
 }
 ```
 #pop-options
 
-// ```pulse
-// fn lookup (#kt:eqtype) (#vt:Type0)
-//   (#pht:erased (pht_t kt vt))
-//   (ht:ht_t kt vt) (k:kt)
-
-//   requires models ht pht
-//   returns  p:(ht_t kt vt & bool & option vt)
-//   ensures  models ht pht ** 
-//            pure (fst p ==> snd p == PHT.lookup pht k)
-
-// {
-//   let p = pulse_lookup_index ht k;
-
-//   if (Mktuple3?._2 p) {
-//     match (Mktuple3?._3 p) {
-//       Some idx -> {
-//         unfold models;
-//         let v = V.op_Array_Access ht.contents idx;
-//         assert (pure (Used? v));
-//         match v {
-//           Used k' v' -> {
-//             assert (pure (k' = k));
-//             fold models;
-//             (true, Some v')
-//           }
-//           _ -> { admit ()  } // why doesn't unreachable() work?
-//         }
-//       }
-//       None -> { (true, None #vt) }
-//     }
-//   } else {
-//     (false, None #vt)
-//   }
-// }
-// ```
-
-// ```pulse
-// fn lookup (#kt:eqtype) (#vt:Type0)
-//   (#ht:erased (ht_t kt vt))
-//   (#pht:erased (pht_t kt vt))
-//   (r:ref (ht_t kt vt)) (k:kt)
-//   requires pts_to r ht ** models ht pht
-//   returns  p:bool & option vt
-//   ensures  pts_to r ht ** models ht pht ** 
-//            pure ( fst p ==> (snd p) == PHT.lookup pht k )
-// {
-//   let res = explode_ref_ht_t r;
-//   match res
-//   {
-//     Mktuple3 r_sz r_hashf r_contents -> {
-//       rewrite (exploded_vp r ht (tfst res) (tsnd res) (tthd res))
-//            as (exploded_vp r ht r_sz r_hashf r_contents);
-//       rewrite (exploded_vp r ht r_sz r_hashf r_contents)
-//            as (exploded_vp (reveal (hide r)) ht r_sz r_hashf r_contents);
-//       let p = pulse_lookup_index (hide r) r_sz r_hashf r_contents k;
-//       rewrite (exploded_vp (reveal (hide r)) ht r_sz r_hashf r_contents)
-//            as (exploded_vp r ht r_sz r_hashf r_contents);
-//       unexplode_ref r r_sz r_hashf r_contents;
-//       if (fst p)
-//       {
-//         match (snd p)
-//         {
-//           Some p -> { (true, Some (fst p)) }
-//           None -> { (true, None #vt) }
-//         }
-//       } 
-//       else
-//       {
-//         (false, None #vt)
-//       }
-//     }
-//   }
-// }
-// ```
-
-
 #restart-solver
-#push-options "--z3rlimit_factor 4 --fuel 1 --ifuel 2"
+#push-options "--fuel 1 --ifuel 2"
 ```pulse
 fn insert (#kt:eqtype) (#vt:Type0)
            (ht:ht_t kt vt) (k:kt) (v:vt)
@@ -379,8 +298,7 @@ fn insert (#kt:eqtype) (#vt:Type0)
   ensures
     exists* pht'.
       models (fst b) pht' **
-      pure ((fst b).sz == ht.sz /\
-            (fst b).hashf == ht.hashf /\
+      pure (same_sz_and_hashf (fst b) ht /\
             (if snd b
              then pht'==PHT.insert pht k v
              else pht'==pht))
@@ -408,7 +326,7 @@ fn insert (#kt:eqtype) (#vt:Type0)
     R.pts_to err verr **
     R.pts_to idx vidx **
     R.pts_to contents vcontents **
-    V.pts_to vcontents s **  // (if (vcont || verr) then pht.repr.seq else (PHT.insert pht k v).repr.seq) **
+    V.pts_to vcontents s **
     pure (
       related ht pht /\
       V.is_full_vec vcontents /\
@@ -417,11 +335,14 @@ fn insert (#kt:eqtype) (#vt:Type0)
       walk pht.repr (SZ.v cidx) k (SZ.v voff) == lookup_repr pht.repr k /\
       insert_repr_walk #kt #vt #(pht_sz pht) #pht.spec pht.repr k v (SZ.v voff) (SZ.v cidx) () () 
         == insert_repr #kt #vt #(pht_sz pht) #pht.spec pht.repr k v /\
-      ((vcont == false /\ verr == false) ==>
+
+      (((not vcont) /\ (not verr)) ==>  // insert succeeded
        (SZ.v vidx < Seq.length s /\
         (insert_repr #kt #vt #(pht_sz pht) #pht.spec pht.repr k v).seq `Seq.equal` 
         Seq.upd s (SZ.v vidx) (mk_used_cell k v))) /\
-      ((vcont == true \/ verr == true) ==> s `Seq.equal` pht.repr.seq) /\
+
+      ((vcont \/ verr) ==> s `Seq.equal` pht.repr.seq) /\  // insert failed
+
       b == (vcont = true && verr = false)
     ))
   {
@@ -439,17 +360,12 @@ fn insert (#kt:eqtype) (#vt:Type0)
         Some sum ->
         {
           let vidx = size_t_mod sum ht.sz;
-          let c = V.replace_ref contents vidx Zombie;
+          let c = V.replace_i_ref contents vidx Zombie;
           match c
           {
             Used k' v' -> {
               if (k' = k) {
-                // assert (pure ( SZ.v idx < Seq.length pht.repr.seq));
-                // V.vec_ref_write contents idx (mk_used_cell k v);
-                // with vcontents. assert (R.pts_to contents vcontents);
-                // with s. assert (V.pts_to vcontents s);
-                // assert (pure (Seq.equal s (Seq.upd pht.repr.seq (SZ.v idx) (mk_used_cell k v))));
-                V.vec_ref_write contents vidx (Used k' v');
+                V.write_ref contents vidx (Used k' v');
                 with vcontents. assert (R.pts_to contents vcontents);
                 with s. assert (V.pts_to vcontents s);
                 assert (pure (Seq.equal s pht.repr.seq));
@@ -458,7 +374,7 @@ fn insert (#kt:eqtype) (#vt:Type0)
                 assert (pure ((insert_repr #kt #vt #(pht_sz pht) #pht.spec pht.repr k v).seq `Seq.equal` 
                               Seq.upd pht.repr.seq (SZ.v vidx) (mk_used_cell k v)));
               } else {
-                V.vec_ref_write contents vidx (Used k' v');
+                V.write_ref contents vidx (Used k' v');
                 with vcontents. assert (R.pts_to contents vcontents);
                 with s. assert (V.pts_to vcontents s);
                 assert (pure (Seq.equal s pht.repr.seq));
@@ -466,14 +382,10 @@ fn insert (#kt:eqtype) (#vt:Type0)
               };
             }
             Clean -> {
-              V.vec_ref_write contents vidx Clean;
+              V.write_ref contents vidx Clean;
               with vcontents. assert (R.pts_to contents vcontents);
               with s. assert (V.pts_to vcontents s);
               assert (pure (Seq.equal s pht.repr.seq));
-              // V.vec_ref_write contents idx (mk_used_cell k v);
-              // with vcontents. assert (R.pts_to contents vcontents);
-              // with s. assert (V.pts_to vcontents s);
-              // assert (pure (Seq.equal s (Seq.upd pht.repr.seq (SZ.v idx) (mk_used_cell k v))));
               cont := false;
               idx := vidx;
               assert (pure ((insert_repr #kt #vt #(pht_sz pht) #pht.spec pht.repr k v).seq `Seq.equal` 
@@ -500,12 +412,10 @@ fn insert (#kt:eqtype) (#vt:Type0)
                 {
                   Some p ->
                   {
-                    (V.vec_ref_write contents p Zombie);
-                    // (V.vec_ref_write contents idx (mk_used_cell k v));
+                    V.write_ref contents p Zombie;
                     with s. rewrite (V.pts_to (reveal (hide (tfst res).contents)) s)
                                as   (V.pts_to (tfst res).contents s);
                     with s. assert (V.pts_to (tfst res).contents s);
-                    // assert (pure (Seq.equal s (Seq.upd (Seq.upd pht.repr.seq (SZ.v (p)) Zombie) (SZ.v idx) (mk_used_cell k v))));
                     cont := false;
                     idx := vidx;
                     assert (pure ((insert_repr #kt #vt #(pht_sz pht) #pht.spec pht.repr k v).seq `Seq.equal` 
@@ -513,11 +423,6 @@ fn insert (#kt:eqtype) (#vt:Type0)
                   }
                   None ->
                   { 
-                    // (V.vec_ref_write contents idx (mk_used_cell k v)); 
-                    // with s. rewrite (V.pts_to (reveal (hide (tfst res).contents)) s)
-                    //            as   (V.pts_to (tfst res).contents s);
-                    // with s. assert (V.pts_to (tfst res).contents s);
-                    // assert (pure (Seq.equal s (Seq.upd pht.repr.seq (SZ.v idx) (mk_used_cell k v))));
                     with s. rewrite (V.pts_to (reveal (hide (tfst res).contents)) s)
                                as   (V.pts_to (tfst res).contents s);
                     with s. assert (V.pts_to (tfst res).contents s);
@@ -552,242 +457,30 @@ fn insert (#kt:eqtype) (#vt:Type0)
   let vidx = !idx;
 
   if (vcont = false && verr = false) {
-    V.vec_ref_write contents vidx (mk_used_cell k v);
+    V.write_ref contents vidx (mk_used_cell k v);
     let vcontents = !contents;
     let ht = mk_ht ht.sz hashf vcontents;
     with vcontents. assert (R.pts_to contents vcontents);
     with s. assert (V.pts_to vcontents s);
     assert (pure (Seq.equal s (PHT.insert pht k v).repr.seq));
     rewrite (V.pts_to vcontents s) as (V.pts_to ht.contents s);
-    let res = (ht, true);
+    let res = ((ht <: ht_t kt vt), true);
     fold (models ht (PHT.insert pht k v));
     with pht. rewrite (models ht pht) as (models (fst res) pht);
-    admit ();
     res
   } else {
     let vcontents = !contents;
     let ht = mk_ht ht.sz hashf vcontents;
-    let res = (ht, false);
+    let res = ((ht <: ht_t kt vt), false);
     with vcontents. assert (R.pts_to contents vcontents);
     with s. assert (V.pts_to vcontents s);
     rewrite (V.pts_to vcontents s) as (V.pts_to ht.contents s);
     fold (models ht pht);
     rewrite (models ht pht) as (models (fst res) pht);
-    admit ();
     res
   }
-
-  // with contents_v_g. assert (R.pts_to contents contents_v_g);
-  // let contents_v = !contents;
-  // let ht = mk_ht ht.sz hashf contents_v;
-  // with s. rewrite (V.pts_to contents_v_g s) as (V.pts_to ht.contents s);
-
-  // let verr = !err;
-  // if verr
-  // {
-  //   let res = (ht, false);
-  //   fold (models ht pht);
-  //   rewrite (models ht pht) as (models (fst res) pht);
-  //   admit ();
-  //   res
-  // } else {
-  //   let res = (ht, true);
-  //   fold (models ht (PHT.insert pht k v));
-  //   with pht. rewrite (models ht pht) as (models (fst res) pht);
-  //   admit ();
-  //   res
-  // }
 }
 ```
-
-// // ```pulse
-// // fn insert (#kt:eqtype) (#vt:Type0)
-// //   (r:ref (ht_t kt vt)) (k:kt) (v:vt)
-// //   (#ht:erased (ht_t kt vt))
-// //   (#pht:(p:erased (pht_t kt vt) { PHT.not_full p.repr }))
-  
-// //   requires pts_to r ht ** models ht pht
-// //   returns b:bool
-// //   ensures exists* pht'.
-// //     pts_to r ht ** models ht pht' **
-// //     pure (if b
-// //           then pht'== PHT.insert pht k v
-// //           else pht'== pht)
-// // {
-// //   let res = explode_ref_ht_t r;
-
-// //   match res {
-
-// //   Mktuple3 r_sz r_hashf r_contents -> {
-// //     rewrite (exploded_vp r ht (tfst res) (tsnd res) (tthd res))
-// //          as (exploded_vp r ht r_sz r_hashf r_contents);
-
-// //     unfold exploded_vp;
-// //     let sz = !r_sz;
-// //     let hash = ref_apply r_hashf k;
-// //     rewrite (R.pts_to r_sz sz) as (R.pts_to r_sz ht.sz);
-// //     fold exploded_vp;
-
-// //     let cidx = size_t_mod hash sz;
-// //     let mut off = 0sz;
-// //     let mut cont = true;
-// //     let mut err = false;
-
-// //     unfold models;
-// //     while
-// //     (
-// //       let vcont = !cont;
-// //       let verr = !err;
-// //       (vcont = true && verr = false)
-// //     ) 
-// //     invariant b. exists* (voff:SZ.t) (vcont verr:bool). (
-// //       exploded_vp r ht r_sz r_hashf r_contents **
-// //       R.pts_to off voff **
-// //       R.pts_to cont vcont **
-// //       R.pts_to err verr **
-// //       V.pts_to ht.contents (if (vcont || verr) then pht.repr.seq else (PHT.insert pht k v).repr.seq) **
-// //       pure (
-// //         related ht pht /\
-// //         SZ.(voff <=^ ht.sz) /\
-// //         strong_all_used_not_by pht.repr (SZ.v cidx) (SZ.v voff) k /\
-// //         walk pht.repr (SZ.v cidx) k (SZ.v voff) == lookup_repr pht.repr k /\
-// //         insert_repr_walk #kt #vt #(pht_sz pht) #pht.spec pht.repr k v (SZ.v voff) (SZ.v cidx) () () 
-// //           == insert_repr #kt #vt #(pht_sz pht) #pht.spec pht.repr k v /\
-// //         b == (vcont = true && verr = false)
-// //       ))
-// //     {
-// //       unfold exploded_vp;
-// //       let voff = !off;
-// //       if (voff = sz)
-// //       {
-// //         cont := false;
-// //         full_not_full pht.repr k;
-// //         assert (V.pts_to ht.contents pht.repr.seq);
-// //         fold exploded_vp;
-// //       }
-// //       else
-// //       {
-// //         let opt_sum = cidx `sz_add` voff;
-// //         match opt_sum
-// //         {
-// //           Some sum ->
-// //           {
-// //             let idx = size_t_mod sum sz;
-// //             rewrite (V.pts_to ht.contents pht.repr.seq)
-// //                  as (V.pts_to (reveal (hide ht.contents)) (reveal (hide pht.repr.seq)));
-// //             let c = V.vec_ref_read r_contents idx;
-// //             rewrite (V.pts_to (reveal (hide ht.contents)) (reveal (hide pht.repr.seq)))
-// //                  as (V.pts_to ht.contents pht.repr.seq);
-
-// //             match c
-// //             {
-// //               Used k' v' -> { 
-// //                 if (k' = k) {
-// //                   assert (V.pts_to ht.contents pht.repr.seq);
-// //                   assert (pure ( SZ.v idx < Seq.length pht.repr.seq));
-// //                   rewrite (V.pts_to ht.contents pht.repr.seq)
-// //                        as (V.pts_to (reveal (hide ht.contents)) (reveal (hide pht.repr.seq)));
-// //                   V.vec_ref_write r_contents idx (mk_used_cell k v);
-// //                   assert (pure ((insert_repr #kt #vt #(pht_sz pht) #pht.spec pht.repr k v).seq `Seq.equal` 
-// //                                 Seq.upd pht.repr.seq (SZ.v idx) (mk_used_cell k v)));
-// //                   rewrite (V.pts_to (reveal (hide ht.contents)) (Seq.upd (reveal (hide pht.repr.seq)) (SZ.v idx) (mk_used_cell k v)))
-// //                        as (V.pts_to ht.contents (insert_repr #kt #vt #(pht_sz pht) #pht.spec pht.repr k v).seq);
-// //                   cont := false;
-// //                   fold exploded_vp;
-// //                 } else {
-// //                   off := SZ.(voff +^ 1sz);
-// //                   fold exploded_vp;
-// //                 } 
-// //               }
-// //               Clean -> {
-// //                 rewrite (V.pts_to ht.contents pht.repr.seq)
-// //                      as (V.pts_to (reveal (hide ht.contents)) (reveal (hide pht.repr.seq)));
-// //                 V.vec_ref_write r_contents idx (mk_used_cell k v);
-// //                 assert (pure ((insert_repr #kt #vt #(pht_sz pht) #pht.spec pht.repr k v).seq `Seq.equal` 
-// //                               Seq.upd pht.repr.seq (SZ.v idx) (mk_used_cell k v)));
-// //                 rewrite (V.pts_to (reveal (hide ht.contents)) (Seq.upd (reveal (hide pht.repr.seq)) (SZ.v idx) (mk_used_cell k v)))
-// //                      as (V.pts_to ht.contents (insert_repr #kt #vt #(pht_sz pht) #pht.spec pht.repr k v).seq);
-// //                 cont := false;
-// //                 fold exploded_vp;
-// //               }
-// //               Zombie ->
-// //               {
-// //                 fold models;
-// //                 fold exploded_vp;
-// //                 rewrite (exploded_vp r ht r_sz r_hashf r_contents)
-// //                      as (exploded_vp (reveal (hide r)) ht r_sz r_hashf r_contents);
-// //                 let lookup_res = pulse_lookup_index (hide r) r_sz r_hashf r_contents k;
-// //                 rewrite (exploded_vp (reveal (hide r)) ht r_sz r_hashf r_contents)
-// //                      as (exploded_vp r ht r_sz r_hashf r_contents);
-// //                 unfold models;
-// //                 unfold exploded_vp;
-
-// //                 if (fst lookup_res)
-// //                 {
-// //                   let o = snd lookup_res;
-// //                   match o
-// //                   {
-// //                     Some p ->
-// //                     {
-// //                       rewrite (V.pts_to ht.contents pht.repr.seq)
-// //                            as (V.pts_to (reveal (hide ht.contents)) (reveal (hide pht.repr.seq)));
-// //                       V.vec_ref_write r_contents (snd p) Zombie;
-// //                       V.vec_ref_write r_contents idx (mk_used_cell k v);
-// //                       cont := false;
-// //                       assert (pure ((insert_repr #kt #vt #(pht_sz pht) #pht.spec pht.repr k v).seq `Seq.equal` 
-// //                                     Seq.upd (Seq.upd pht.repr.seq (SZ.v (snd p)) Zombie) (SZ.v idx) (mk_used_cell k v)));
-// //                       rewrite (V.pts_to (reveal (hide ht.contents))
-// //                                         (Seq.upd (Seq.upd (reveal (hide pht.repr.seq)) (SZ.v (snd p)) Zombie) (SZ.v idx) (mk_used_cell k v)))
-// //                            as (V.pts_to ht.contents (insert_repr #kt #vt #(pht_sz pht) #pht.spec pht.repr k v).seq);
-// //                       fold exploded_vp;
-// //                     }
-// //                     None ->
-// //                     {
-// //                       rewrite (V.pts_to ht.contents pht.repr.seq)
-// //                            as (V.pts_to (reveal (hide ht.contents)) (reveal (hide pht.repr.seq)));
-// //                       V.vec_ref_write r_contents idx (mk_used_cell k v);                    
-// //                       cont := false;
-// //                       assert (pure ((insert_repr #kt #vt #(pht_sz pht) #pht.spec pht.repr k v).seq `Seq.equal`
-// //                                     Seq.upd pht.repr.seq (SZ.v idx) (mk_used_cell k v)));
-// //                       rewrite (V.pts_to (reveal (hide ht.contents)) (Seq.upd (reveal (hide pht.repr.seq)) (SZ.v idx) (mk_used_cell k v)))
-// //                            as (V.pts_to ht.contents (insert_repr #kt #vt #(pht_sz pht) #pht.spec pht.repr k v).seq);
-// //                       fold exploded_vp;
-// //                     }
-// //                   }
-// //                 }
-// //                 else
-// //                 {
-// //                   // ERROR - lookup failed
-// //                   err := true;
-// //                   fold exploded_vp;
-// //                 }
-// //               }
-// //             }
-// //           }
-// //           None ->
-// //           {
-// //             // ERROR - add failed
-// //             err := true;
-// //             fold exploded_vp;
-// //           }
-// //         }
-// //       }
-// //     };
-// //     unexplode_ref r r_sz r_hashf r_contents;
-// //     let verr = !err;
-// //     if verr
-// //     {
-// //       fold (models ht pht);
-// //       false
-// //     } else {
-// //       assert (V.pts_to ht.contents (PHT.insert pht k v).repr.seq);
-// //       fold (models ht (PHT.insert pht k v));
-// //       true
-// //     }
-// //     }
-// //   }
-// // }
-// // ```
 
 ```pulse
 fn delete (#kt:eqtype) (#vt:Type0)
@@ -799,8 +492,7 @@ fn delete (#kt:eqtype) (#vt:Type0)
   ensures
     (exists* pht'. 
      models (fst b) pht' **
-     pure ((fst b).sz == ht.sz /\
-           (fst b).hashf == ht.hashf /\
+     pure (same_sz_and_hashf (fst b) ht /\
            (if snd b then pht' == PHT.delete pht k else pht' == pht)))
 {
   let hashf = ht.hashf;
@@ -813,7 +505,7 @@ fn delete (#kt:eqtype) (#vt:Type0)
   let mut cont = true;
   let mut err = false;
 
-  while 
+  while
   (
     let vcont = !cont;
     let verr = !err; 
@@ -849,14 +541,14 @@ fn delete (#kt:eqtype) (#vt:Type0)
         Some sum ->
         {
           let idx = size_t_mod sum ht.sz;
-          let c = V.vec_ref_read contents idx;
+          let c = V.read_ref contents idx;
           match c
           {
             Used k' v' ->
             { 
               if (k' = k)
               {
-                V.vec_ref_write contents idx Zombie;
+                V.write_ref contents idx Zombie;
                 cont := false;
                 assert (pure (pht.repr @@ SZ.v idx == Used k v'));
                 assert (pure (Seq.upd pht.repr.seq (SZ.v idx) Zombie 
@@ -895,166 +587,27 @@ fn delete (#kt:eqtype) (#vt:Type0)
   let verr = !err;
   if verr
   {
-    let res = (ht, false);
+    let res = ((ht <: ht_t kt vt), false);
     fold (models ht pht);
     rewrite (models ht pht) as (models (fst res) pht);
-    admit ();
     res
   }
   else
   {
-    let res = (ht, true);
+    let res = ((ht <: ht_t kt vt), true);
     fold (models ht (PHT.delete pht k));
     rewrite (models ht (PHT.delete pht k)) as (models (fst res) (PHT.delete pht k));
-    admit ();
     res
   }
 }
 ```
 
-// // ```pulse
-// // fn delete (#kt:eqtype) (#vt:Type0)
-// //   (r:ref (ht_t kt vt)) (k:kt)
-// //   (#ht:erased (ht_t kt vt))
-// //   (#pht:erased (pht_t kt vt))
-// //   requires pts_to r ht ** models ht pht
-// //   returns b:bool
-// //   ensures exists* pht'.
-// //     pts_to r ht **
-// //     models ht pht' **
-// //     pure (if b then pht' == PHT.delete pht k else pht' == pht)
-// // {
-// //   let res = explode_ref_ht_t r;
-
-// //   match res {
-
-// //   Mktuple3 r_sz r_hashf r_contents -> {
-// //   rewrite (exploded_vp r ht (tfst res) (tsnd res) (tthd res))
-// //        as (exploded_vp r ht r_sz r_hashf r_contents);
-  
-// //   unfold exploded_vp;
-// //   let sz = !r_sz;
-// //   let hash = ref_apply r_hashf k;
-// //   rewrite (pts_to r_sz sz) as (pts_to r_sz ht.sz);
-// //   fold exploded_vp;
-
-// //   let cidx = size_t_mod hash sz;
-// //   let mut off = 0sz;
-// //   let mut cont = true;
-// //   let mut err = false;
-
-// //   unfold models;
-// //   while 
-// //   (
-// //     let vcont = !cont;
-// //     let verr = !err; 
-// //     (vcont = true && verr = false)
-// //   )
-// //   invariant b. exists* (voff:SZ.t) (vcont verr:bool). (
-// //     exploded_vp r ht r_sz r_hashf r_contents **
-// //     R.pts_to off voff **
-// //     R.pts_to cont vcont **
-// //     R.pts_to err verr **
-// //     V.pts_to ht.contents (if (vcont || verr) then pht.repr.seq else (PHT.delete pht k).repr.seq) **
-// //     pure (
-// //       SZ.v ht.sz == pht_sz pht /\
-// //       SZ.(voff <=^ ht.sz) /\
-// //       all_used_not_by pht.repr (SZ.v cidx) (SZ.v voff) k /\
-// //       walk pht.repr (SZ.v cidx) k (SZ.v voff) == lookup_repr pht.repr k /\
-// //       delete_repr_walk #kt #vt #(pht_sz pht) #pht.spec pht.repr k (SZ.v voff) (SZ.v cidx) () () 
-// //         == delete_repr #kt #vt #(pht_sz pht) #pht.spec pht.repr k /\
-// //       b == (vcont = true && verr = false)
-// //     ))
-// //   {
-// //     unfold exploded_vp;
-// //     let voff = !off;
-// //     if (voff = sz)
-// //     {
-// //       cont := false;
-// //       assert (V.pts_to ht.contents pht.repr.seq);
-// //       fold exploded_vp;
-// //     }
-// //     else
-// //     {
-// //       let opt_sum = cidx `sz_add` voff;
-// //       match opt_sum
-// //       {
-// //         Some sum ->
-// //         {
-// //           let idx = size_t_mod sum sz;
-// //           rewrite (V.pts_to ht.contents pht.repr.seq)
-// //                as (V.pts_to (reveal (hide ht.contents)) (reveal (hide pht.repr.seq)));
-// //           let c = V.vec_ref_read r_contents idx;
-// //           rewrite (V.pts_to (reveal (hide ht.contents)) (reveal (hide pht.repr.seq)))
-// //                as (V.pts_to ht.contents pht.repr.seq);
-
-// //           match c
-// //           {
-// //             Used k' v' ->
-// //             { 
-// //               if (k' = k)
-// //               {
-// //                 rewrite (V.pts_to ht.contents pht.repr.seq)
-// //                      as (V.pts_to (reveal (hide ht.contents)) (reveal (hide pht.repr.seq)));
-// //                 V.vec_ref_write r_contents idx Zombie;
-// //                 cont := false;
-// //                 assert (pure (pht.repr @@ SZ.v idx == Used k v'));
-// //                 assert (pure (Seq.upd pht.repr.seq (SZ.v idx) Zombie  `Seq.equal`
-// //                               (PHT.delete pht k).repr.seq));
-// //                 rewrite (V.pts_to (reveal (hide ht.contents)) (Seq.upd (reveal (hide pht.repr.seq)) (SZ.v idx) Zombie))
-// //                      as (V.pts_to ht.contents (PHT.delete pht k).repr.seq);
-// //                 fold exploded_vp;
-// //               }
-// //               else
-// //               {
-// //                 off := SZ.(voff +^ 1sz);
-// //                 fold exploded_vp;
-// //               } 
-// //             }
-// //             Clean ->
-// //             {
-// //               cont := false;
-// //               assert (pure (pht.repr == (PHT.delete pht k).repr));
-// //               fold exploded_vp;
-// //             }
-// //             Zombie ->
-// //             {
-// //               off := SZ.(voff +^ 1sz);
-// //               fold exploded_vp;
-// //             }
-// //           }
-// //         }
-// //         None ->
-// //         {
-// //           // ERROR - add failed
-// //           err := false;
-// //           fold exploded_vp;
-// //         }
-// //       }
-// //     }
-// //   };
-// //   unexplode_ref r r_sz r_hashf r_contents;
-// //   let verr = !err;
-// //   if verr
-// //   {
-// //     fold (models ht pht);
-// //     false
-// //   }
-// //   else
-// //   {
-// //     fold (models ht (PHT.delete pht k));
-// //     true
-// //   }
-// //   }
-// //   }
-// // }
-// // ```
-
-let is_used (#k:eqtype) (#v:Type0) (c:cell k v) : (p:(bool & cell k v){snd p == c}) =
+let is_used (#k:eqtype) (#v:Type0) (c:cell k v) : (bool & cell k v) =
   match c with
   | Used _ _ -> true, c
   | _ -> false, c
 
+#push-options "--print_implicits"
 ```pulse
 fn not_full (#kt:eqtype) (#vt:Type0)
   (ht:ht_t kt vt)
@@ -1064,22 +617,22 @@ fn not_full (#kt:eqtype) (#vt:Type0)
   returns b:(ht_t kt vt & bool)
   ensures
     models (fst b) pht ** 
-    pure ((fst b).sz == ht.sz /\ (fst b).hashf == ht.hashf /\ (snd b ==> PHT.not_full pht.repr))
+    pure (same_sz_and_hashf (fst b) ht /\ (snd b ==> PHT.not_full pht.repr))
 {
   let hashf = ht.hashf;
   let mut contents = ht.contents;
 
   let mut i = 0sz;
   unfold (models ht pht);
-  // with s. rewrite (V.pts_to ht.contents s) as (V.pts_to contents s);
+
   while
   (
     let vi = !i;  
     if SZ.(vi <^ ht.sz) 
     { 
-      let c = V.replace_ref contents vi Zombie;
+      let c = V.replace_i_ref contents vi Zombie;
       let b = is_used c;
-      V.replace_ref contents vi (snd b);
+      V.replace_i_ref contents vi (snd b);
       with vcontents. assert (R.pts_to contents vcontents);
       with s. assert (V.pts_to vcontents s);
       assert (pure (Seq.equal s pht.repr.seq));
@@ -1115,130 +668,46 @@ fn not_full (#kt:eqtype) (#vt:Type0)
   with vcontentsg. assert (R.pts_to contents vcontentsg);
   with s. rewrite (V.pts_to vcontentsg s) as (V.pts_to ht.contents s);
   fold (models ht pht);
-  let b = (ht, res);
+  let b = ((ht <: ht_t kt vt), (res <: bool));
   rewrite (models ht pht) as (models (fst b) pht);
-  admit ();
   b
-  // let vi = !i;
-  // let res = SZ.(vi <^ ht.sz);
-  // with s. rewrite (V.pts_to contents s) as (V.pts_to ht.contents s);
-  // fold (models ht pht);
-  // let ht = mk_ht ht.sz hashf contents;
-  // (ht, res)
 }
 ```
 
-// // ```pulse
-// // fn not_full (#kt:eqtype) (#vt:Type0)
-// //   (r:ref (ht_t kt vt))
-// //   (#ht:erased (ht_t kt vt))
-// //   (#pht:erased (pht_t kt vt))
-// //   requires pts_to r ht ** models ht pht
-// //   returns b:bool
-// //   ensures pts_to r ht ** models ht pht ** 
-// //           pure (b ==> PHT.not_full pht.repr)
-// // {
-// //   let res = explode_ref_ht_t r;
-
-// //   match res {
- 
-// //   Mktuple3 r_sz r_hashf r_contents -> {
-
-// //   rewrite (exploded_vp r ht (tfst res) (tsnd res) (tthd res))
-// //        as (exploded_vp r ht r_sz r_hashf r_contents);
-
-// //   let mut i = 0sz;
-// //   unfold models;
-
-// //   unfold exploded_vp;
-// //   let sz = !r_sz;
-// //   rewrite (R.pts_to r_sz sz) as (R.pts_to r_sz ht.sz);
-// //   fold exploded_vp;
-
-// //   while
-// //   (
-// //     let vi = !i;  
-// //     if SZ.(vi <^ sz)
-// //     {
-// //       unfold exploded_vp;
-// //       rewrite (V.pts_to ht.contents pht.repr.seq)
-// //            as (V.pts_to (reveal (hide ht.contents)) (reveal (hide pht.repr.seq)));
-// //       let c = V.vec_ref_read r_contents vi;
-// //       rewrite (V.pts_to (reveal (hide ht.contents)) (reveal (hide pht.repr.seq)))
-// //            as (V.pts_to ht.contents pht.repr.seq);
-// //       fold exploded_vp;
-// //       is_used c
-// //     }
-// //     else 
-// //     { 
-// //       false
-// //     }
-// //   )
-// //   invariant b. exists* (vi:SZ.t). (
-// //     exploded_vp r ht r_sz r_hashf r_contents **
-// //     V.pts_to ht.contents pht.repr.seq **
-// //     R.pts_to i vi **
-// //     pure (
-// //       SZ.v ht.sz == pht_sz pht /\
-// //       SZ.(vi <=^ ht.sz) /\
-// //       (b == (SZ.(vi <^ ht.sz) && Used? (pht.repr @@ (SZ.v vi)))) /\
-// //       (forall (i:nat). i < SZ.v vi ==> is_used (pht.repr @@ i))
-// //     )
-// //   )
-// //   {
-// //     let vi = !i;
-// //     i := SZ.(vi +^ 1sz);
-// //   };
-// //   unexplode_ref r r_sz r_hashf r_contents;
-// //   let vi = !i;
-// //   let res = SZ.(vi <^ sz);
-// //   fold models;
-// //   res
-// // }
-// // }
-// // }
-// // ```
-
-// let hash_us (k:SZ.t) : SZ.t = k
-
-// let init_not_full (#kt:eqtype) (#vt:eqtype) (hashf:kt -> SZ.t) (l:pos_us)
-//   : Lemma (Pulse.Lib.HashTable.Spec.not_full (mk_init_pht #kt #vt hashf l).repr)
-//   = assert (~(Used? ((mk_init_pht #kt #vt hashf l).repr @@ 0)))
-
-// // ```pulse
-// // fn test_mono ()
-// //   requires emp
-// //   ensures emp
-// // {
-// //    let htc = alloc #SZ.t #SZ.t hash_us 128sz;
-// //    with pht. assert (models htc pht);
-// //    let ht = R.alloc htc;
-// //    init_not_full #SZ.t #SZ.t hash_us 128sz;
-// //    rewrite (models htc pht) as (models (reveal (hide htc)) pht);
-// //    let b = insert ht 0sz 17sz;
-// //    if (b) {
-// //      let v = lookup ht 0sz;
-// //      if (fst v) {
-// //        assert pure (snd v == Some 17sz);
-// //        R.free ht;
-// //        with pht. assert (models (reveal (hide htc)) pht);
-// //        rewrite (models (reveal (hide htc)) pht) as (models htc pht);
-// //        dealloc htc
-// //      }
-// //      else {
-// //       R.free ht;
-// //       with pht. assert (models (reveal (hide htc)) pht);
-// //       rewrite (models (reveal (hide htc)) pht) as (models htc pht);
-// //       dealloc htc
-// //      }
-// //    }
-// //    else {
-// //     let b = delete ht 0sz;
-// //     let b' = not_full ht;
-// //     R.free ht;
-// //     with pht. assert (models (reveal (hide htc)) pht);
-// //     rewrite (models (reveal (hide htc)) pht) as (models htc pht);
-// //     dealloc htc
-// //    } 
-// // }
-// // ```
+// ```pulse
+// fn test_mono ()
+//   requires emp
+//   ensures emp
+// {
+//    let htc = alloc #SZ.t #SZ.t hash_us 128sz;
+//    with pht. assert (models htc pht);
+//    let ht = R.alloc htc;
+//    init_not_full #SZ.t #SZ.t hash_us 128sz;
+//    rewrite (models htc pht) as (models (reveal (hide htc)) pht);
+//    let b = insert ht 0sz 17sz;
+//    if (b) {
+//      let v = lookup ht 0sz;
+//      if (fst v) {
+//        assert pure (snd v == Some 17sz);
+//        R.free ht;
+//        with pht. assert (models (reveal (hide htc)) pht);
+//        rewrite (models (reveal (hide htc)) pht) as (models htc pht);
+//        dealloc htc
+//      }
+//      else {
+//       R.free ht;
+//       with pht. assert (models (reveal (hide htc)) pht);
+//       rewrite (models (reveal (hide htc)) pht) as (models htc pht);
+//       dealloc htc
+//      }
+//    }
+//    else {
+//     let b = delete ht 0sz;
+//     let b' = not_full ht;
+//     R.free ht;
+//     with pht. assert (models (reveal (hide htc)) pht);
+//     rewrite (models (reveal (hide htc)) pht) as (models htc pht);
+//     dealloc htc
+//    } 
+// }
+// ```
