pulse/share/steel/examples/pulse/dice/engine/EngineTypes.fst
@@ -15,12 +15,6 @@
 *)
 
 module EngineTypes
-open Pulse.Lib.Pervasives
-module R = Pulse.Lib.Reference
-module A = Pulse.Lib.Array
-module US = FStar.SizeT
-module U8 = FStar.UInt8
-open HACL
 
 let uds_is_enabled : vprop 
 = admit()
