pulse/share/steel/examples/pulse/dice/l0/L0Types.fsti
@@ -17,7 +17,7 @@
 module L0Types
 open Pulse.Lib.Pervasives
 module R = Pulse.Lib.Reference
-module A = Pulse.Lib.Array
+module V = Pulse.Lib.Vec
 module US = FStar.SizeT
 module U8 = FStar.UInt8
 module U32 = FStar.UInt32
@@ -63,11 +63,11 @@ type aliasKeyCRT_ingredients_t = {
 (* Record *)
 noeq
 type l0_record_t = {
-  fwid: A.larray U8.t (US.v v32us);
+  fwid: V.lvec U8.t (US.v v32us);
   deviceID_label_len: hkdf_lbl_len;
-  deviceID_label: A.larray U8.t (US.v deviceID_label_len); (* public bytes *)
+  deviceID_label: V.lvec U8.t (US.v deviceID_label_len); (* public bytes *)
   aliasKey_label_len: hkdf_lbl_len;
-  aliasKey_label: A.larray U8.t (US.v aliasKey_label_len); (* public bytes *)
+  aliasKey_label: V.lvec U8.t (US.v aliasKey_label_len); (* public bytes *)
   deviceIDCSR_ingredients: deviceIDCSR_ingredients_t;
   aliasKeyCRT_ingredients: aliasKeyCRT_ingredients_t;
 }
@@ -84,9 +84,9 @@ let mk_l0_repr fwid deviceID_label aliasKey_label
 
 // don't need full perm
 let l0_record_perm (record:l0_record_t) (p:perm) (repr:l0_record_repr_t) : vprop =
-  A.pts_to record.fwid #p repr.fwid **
-  A.pts_to record.deviceID_label #p repr.deviceID_label **
-  A.pts_to record.aliasKey_label #p repr.aliasKey_label **
+  V.pts_to record.fwid #p repr.fwid **
+  V.pts_to record.deviceID_label #p repr.deviceID_label **
+  V.pts_to record.aliasKey_label #p repr.aliasKey_label **
   pure (
     valid_hkdf_lbl_len record.deviceID_label_len /\
     valid_hkdf_lbl_len record.aliasKey_label_len
