pulse/share/steel/examples/pulse/lib/Pulse.Lib.Vec.fsti
@@ -31,6 +31,8 @@ val vec ([@@@strictly_positive] a:Type0) : Type u#0
 
 val length (#a:Type0) (v:vec a) : GTot nat
 
+type lvec (a:Type0) (n:nat) = v:vec a { length v == n }
+
 val is_full_vec (#a:Type0) (v:vec a) : prop
 
 val pts_to (#a:Type0) (v:vec a) (#[T.exact (`full_perm)] p:perm) (s:Seq.seq a) : vprop
@@ -115,7 +117,7 @@ val to_vec_pts_to (#a:Type0) (v:vec a) (#p:perm) (#s:Seq.seq a)
       (A.pts_to (vec_to_array v) #p s)
       (fun _ → pts_to v #p s)
 
-val vec_ref_read (#a:Type0) (r:R.ref (vec a))
+val read_ref (#a:Type0) (r:R.ref (vec a))
   (i:SZ.t)
   (#v:erased (vec a))
   (#s:erased (Seq.seq a) { SZ.v i < Seq.length s})
@@ -123,7 +125,7 @@ val vec_ref_read (#a:Type0) (r:R.ref (vec a))
     (requires R.pts_to r v ** pts_to v s)
     (ensures fun res -> R.pts_to r v ** pts_to v s ** pure (res == Seq.index s (SZ.v i)))
 
-val vec_ref_write (#a:Type0) (r:R.ref (vec a))
+val write_ref (#a:Type0) (r:R.ref (vec a))
   (i:SZ.t)
   (x:a)
   (#v:erased (vec a))
@@ -132,23 +134,15 @@ val vec_ref_write (#a:Type0) (r:R.ref (vec a))
     (requires R.pts_to r v ** pts_to v s)
     (ensures fun _ -> R.pts_to r v ** pts_to v (Seq.upd s (SZ.v i) x))
 
-val replace (#a:Type0) (v:vec a) (i:SZ.t) (x:a)
+val replace_i (#a:Type0) (v:vec a) (i:SZ.t) (x:a)
   (#s:erased (Seq.seq a) { SZ.v i < Seq.length s})
   : stt a
     (requires pts_to v s)
     (ensures fun res -> pts_to v (Seq.upd s (SZ.v i) x) ** pure (res == Seq.index s (SZ.v i)))
 
-val replace_ref (#a:Type0) (r:R.ref (vec a)) (i:SZ.t) (x:a)
+val replace_i_ref (#a:Type0) (r:R.ref (vec a)) (i:SZ.t) (x:a)
   (#v:erased (vec a))
   (#s:erased (Seq.seq a) { SZ.v i < Seq.length s})
   : stt a
     (requires R.pts_to r v ** pts_to v s)
     (ensures fun res -> R.pts_to r v ** pts_to v (Seq.upd s (SZ.v i) x) ** pure (res == Seq.index s (SZ.v i)))
-
-val copy (#a:Type0) (v_dst v_src:vec a) (len:SZ.t)
-  (#p_src:perm)
-  (#s_src:erased (Seq.seq a) { SZ.v len == Seq.length s_src })
-  (#s_dst:erased (Seq.seq a) { Seq.length s_dst == Seq.length s_dst })
-  : stt unit
-      (requires pts_to v_src #p_src s_src ** pts_to v_dst s_dst)
-      (ensures fun _ -> pts_to v_src #p_src s_src ** pts_to v_dst s_src)
